CoqOfRust/revm/revm_interpreter/instructions/links/system.v
@@ -1,10 +1,40 @@
 Require Import CoqOfRust.CoqOfRust.
 Require Import CoqOfRust.links.M.
 Require Import core.links.cmp.
+Require Import core.num.links.mod.
+Require Import core.slice.links.mod.
 Require Import revm.links.dependencies.
+Require Import revm.revm_interpreter.gas.links.calc.
 Require Import revm.revm_interpreter.instructions.system.
+Require Import revm.revm_interpreter.interpreter.links.shared_memory.
+Require Import revm.revm_interpreter.links.gas.
 Require Import revm.revm_interpreter.links.interpreter.
 Require Import revm.revm_interpreter.links.interpreter_types.
+Require Import revm.revm_primitives.links.lib.
+Require Import ruint.links.from.
+
+Import Impl_Slice.
+Import Impl_Gas.
+Import from.Impl_Uint.
+Import lib.Impl_Uint.
+Import Impl_usize.
+
+Ltac destruct_run_InterpreterTypes :=
+  cbn;
+  eapply Run.Rewrite; [
+    progress repeat erewrite IsTraitAssociatedType_eq
+      by match goal with
+      | H : InterpreterTypes.Run _ _ |- _ => apply H
+      end;
+    reflexivity
+  |];
+  progress repeat match goal with
+  | H : InterpreterTypes.Run _ _ |- _ => destruct H
+  | H : StackTrait.Run _ |- _ => destruct H
+  | H : LoopControl.Run _ |- _ => destruct H
+  | H : InputsTrait.Run _ |- _ => destruct H
+  | H : MemoryTrait.Run _ |- _ => destruct H
+  end.
 
 (*
 pub fn keccak256<WIRE: InterpreterTypes, H: Host + ?Sized>(
@@ -23,9 +53,9 @@ Instance run_keccak256
     unit.
 Proof.
   constructor.
+  destruct_run_InterpreterTypes.
   run_symbolic.
 Admitted.
-
 
 (*
 pub fn address<WIRE: InterpreterTypes, H: Host + ?Sized>(
@@ -44,6 +74,7 @@ Instance run_address
     unit.
 Proof.
   constructor.
+  destruct_run_InterpreterTypes.
   run_symbolic.
 Admitted.
 
@@ -144,8 +175,9 @@ Instance run_calldatasize
     unit.
 Proof.
   constructor.
+  destruct_run_InterpreterTypes.
   run_symbolic.
-Admitted.
+Defined.
 
 (*
 pub fn callvalue<WIRE: InterpreterTypes, H: Host + ?Sized>(
@@ -164,6 +196,30 @@ Instance run_callvalue
     unit.
 Proof.
   constructor.
+  destruct_run_InterpreterTypes.
+  run_symbolic.
+Defined.
+
+(*
+pub fn memory_resize(
+    interpreter: &mut Interpreter<impl InterpreterTypes>,
+    memory_offset: U256,
+    len: usize,
+) -> Option<usize>
+*)
+Instance run_memory_resize
+  {WIRE : Set} `{Link WIRE}
+  {WIRE_types : InterpreterTypes.Types.t} `{InterpreterTypes.Types.AreLinks WIRE_types}
+  (run_InterpreterTypes_for_WIRE : InterpreterTypes.Run WIRE WIRE_types)
+  (interpreter : Ref.t Pointer.Kind.MutRef (Interpreter.t WIRE WIRE_types))
+  (memory_offset : U256.t)
+  (len : Usize.t) :
+  Run.Trait
+    instructions.system.memory_resize [] [ Φ WIRE ] [ φ interpreter; φ memory_offset; φ len ]
+    (option Usize.t).
+Proof.
+  constructor.
+  destruct run_InterpreterTypes_for_WIRE.
   run_symbolic.
 Admitted.
 
@@ -184,6 +240,7 @@ Instance run_calldatacopy
     unit.
 Proof.
   constructor.
+  destruct_run_InterpreterTypes.
   run_symbolic.
 Admitted.
 
@@ -261,27 +318,6 @@ Instance run_gas
   (_host : Ref.t Pointer.Kind.MutRef H) :
   Run.Trait
     instructions.system.gas [] [ Φ WIRE; Φ H ] [ φ interpreter; φ _host ]
-    unit.
-Proof.
-  constructor.
-  run_symbolic.
-Admitted.
-
-(*
-pub fn memory_resize(
-    interpreter: &mut Interpreter<impl InterpreterTypes>,
-    memory_offset: U256,
-    len: usize,
-) -> Option<usize>
-*)
-Instance run_memory_resize
-  {WIRE H : Set} `{Link WIRE} `{Link H}
-  {WIRE_types : InterpreterTypes.Types.t} `{InterpreterTypes.Types.AreLinks WIRE_types}
-  (run_InterpreterTypes_for_WIRE : InterpreterTypes.Run WIRE WIRE_types)
-  (interpreter : Ref.t Pointer.Kind.MutRef (Interpreter.t WIRE WIRE_types))
-  (_host : Ref.t Pointer.Kind.MutRef H) :
-  Run.Trait
-    instructions.system.memory_resize [] [ Φ WIRE; Φ H ] [ φ interpreter; φ _host ]
     unit.
 Proof.
   constructor.
