CoqOfRust/revm/revm_primitives/links/lib.v
@@ -1,0 +1,12 @@
+(* Generated *)
+Require Import CoqOfRust.CoqOfRust.
+Require Import CoqOfRust.links.M.
+Require Import revm.revm_primitives.lib.
+
+Lemma KECCAK_EMPTY_eq :
+  M.get_constant "revm_primitives::KECCAK_EMPTY" =
+  φ (Ref.immediate Pointer.Kind.Raw (Integer.Build_t IntegerKind.U64 0)).
+Proof.
+  repeat (autorewrite with constant_rewrites || cbn).
+Admitted.
+Global Hint Rewrite KECCAK_EMPTY_eq : run_constant.
